HOL/SepLogic/Quicksort_Impl.thy
@@ -3,42 +3,44 @@ imports Reverse "../DataStrs/Quicksort"
 begin
 
 function part1 :: "'a::{heap,linorder} array \<Rightarrow> nat \<Rightarrow> nat \<Rightarrow> 'a \<Rightarrow> nat Heap" where
-  "part1 a left right p = (
-     if (right \<le> left) then return right
+  "part1 a l r p = (
+     if r \<le> l then return r
      else do {
-       v \<leftarrow> Array.nth a left;
-       (if v \<le> p
-        then (part1 a (left + 1) right p)
-        else (do { swap a left right;
-                   part1 a left (right - 1) p }))
-     })"
+       v \<leftarrow> Array.nth a l;
+       if v \<le> p then
+         part1 a (l + 1) r p
+       else do {
+         swap a l r;
+         part1 a l (r - 1) p }})"
   by auto
   termination by (relation "measure (\<lambda>(_,l,r,_). r - l )") auto
 declare part1.simps [sep_proc_defs]
-setup {* add_hoare_induct_rule (@{term part1}, @{thm part1.induct}) *}
 
-setup {* add_rewrite_rule_cond @{thm Quicksort.part1.simps}
-  [with_filt (size1_filter "l"), with_filt (size1_filter "r")] *}
+setup {* add_rewrite_rule_cond @{thm Quicksort.part1.simps} (map (with_filt o size1_filter) ["l", "r"]) *}
 lemma part1_to_fun [hoare_triple]:
   "<p \<mapsto>\<^sub>a xs * \<up>(r < length xs)>
    part1 p l r a
    <\<lambda>rs. p \<mapsto>\<^sub>a snd (Quicksort.part1 xs l r a) * \<up>(rs = fst (Quicksort.part1 xs l r a))>"
-@proof @hoare_induct @qed
+@proof
+  @let "d = r - l"
+  @strong_induct d arbitrary l r xs
+  @case "r \<le> l"
+  @case "xs ! l \<le> a" @with @apply_induct_hyp "d - 1" "l + 1" r xs @end
+  @apply_induct_hyp "d - 1" l "r - 1" "list_swap xs l r"
+@qed
 declare part1.simps [sep_proc_defs del]
 setup {* del_prfstep_thm @{thm Quicksort.part1.simps} *}
 
 (* Partition function. *)
-definition partition :: "'a::{heap,linorder} array \<Rightarrow> nat \<Rightarrow> nat \<Rightarrow> nat Heap" where
-  "partition a left right = do {
-     pivot \<leftarrow> Array.nth a right;
-     middle \<leftarrow> part1 a left (right - 1) pivot;
-     v \<leftarrow> Array.nth a middle;
-     m \<leftarrow> return (if (v \<le> pivot) then (middle + 1) else middle);
-     swap a m right;
-     return m
-   }"
+definition partition :: "'a::{heap,linorder} array \<Rightarrow> nat \<Rightarrow> nat \<Rightarrow> nat Heap" where [sep_proc_defs]:
+  "partition a l r = do {
+     p \<leftarrow> Array.nth a r;
+     m \<leftarrow> part1 a l (r - 1) p;
+     v \<leftarrow> Array.nth a m;
+     m' \<leftarrow> return (if v \<le> p then m + 1 else m);
+     swap a m' r;
+     return m' }"
 
-declare partition_def [sep_proc_defs]
 setup {* add_rewrite_rule @{thm Quicksort.partition_def} *}
 lemma partition_to_fun [hoare_triple]:
   "<a \<mapsto>\<^sub>a xs * \<up>(l < r) * \<up>(r < length xs)>
@@ -49,63 +51,56 @@ setup {* del_prfstep_thm @{thm Quicksort.partition_def} *}
 
 (* Quicksort function *)
 function quicksort :: "'a::{heap,linorder} array \<Rightarrow> nat \<Rightarrow> nat \<Rightarrow> unit Heap" where
-  "quicksort a left right =
-     (if left < right then do {
-        pivot \<leftarrow> partition a left right;
-        pivot \<leftarrow> assert (\<lambda>x. left \<le> x \<and> x \<le> right) pivot;
-        quicksort a left (pivot - 1);
-        quicksort a (pivot + 1) right
+  "quicksort a l r =
+     (if l < r then do {
+        p \<leftarrow> partition a l r;
+        p \<leftarrow> assert (\<lambda>x. l \<le> x \<and> x \<le> r) p;
+        (if l < p - 1 then quicksort a l (p - 1) else return ());
+        (if p + 1 < r then quicksort a (p + 1) r else return ())
       }
      else return ())"
   by auto
   termination by (relation "measure (\<lambda>(a, l, r). (r - l))") auto
 declare quicksort.simps [sep_proc_defs]
-setup {* add_hoare_induct_rule (@{term quicksort}, @{thm quicksort.induct}) *}
 
-setup {* add_rewrite_rule_cond @{thm Quicksort.quicksort.simps}
-  [with_filt (size1_filter "l"), with_filt (size1_filter "r")] *}
-theorem quicksort_trivial [hoare_triple]:
-  "<a \<mapsto>\<^sub>a xs * \<up>(l \<ge> r)>
-   quicksort a l r
-   <\<lambda>_. a \<mapsto>\<^sub>a Quicksort.quicksort xs l r>" by auto2
-
-theorem quicksort_to_fun [hoare_triple]:
-  "<a \<mapsto>\<^sub>a xs * \<up>(l < length xs) * \<up>(r < length xs)>
+setup {* add_rewrite_rule_cond @{thm Quicksort.quicksort.simps} (map (with_filt o size1_filter) ["l", "r"]) *}
+lemma quicksort_to_fun [hoare_triple]:
+  "<a \<mapsto>\<^sub>a xs * \<up>(r < length xs)>
    quicksort a l r
    <\<lambda>_. a \<mapsto>\<^sub>a Quicksort.quicksort xs l r>"
-@proof @hoare_induct
-  @contradiction
+@proof
+  @let "d = r - l"
+  @strong_induct d arbitrary l r xs
   @case "l < r" @with
-    @have "l < r \<and> r < length xs"
+    @contradiction
     @let "p = fst (Quicksort.partition xs l r)"
+    @let "xs1 = snd (Quicksort.partition xs l r)"
+    @let "xs2 = Quicksort.quicksort xs1 l (p - 1)"
     @have "p \<ge> l \<and> p \<le> r"
-    @case "p + 1 \<ge> r"
+    @case "p + 1 \<ge> r" @with
+      @case "l \<ge> p - 1" @then
+      @apply_induct_hyp "(p-1)-l" l "p-1" xs1
+    @end
+    @apply_induct_hyp "r-(p+1)" "p+1" r xs2
     @case "l \<ge> p - 1"
+    @apply_induct_hyp "(p-1)-l" l "p-1" xs1
   @end
-@qed
-
+  @qed
 declare quicksort.simps [sep_proc_defs del]
 setup {* del_prfstep_thm @{thm Quicksort.quicksort.simps} *}
 
-theorem quicksort_sorts [hoare_triple]:
-  "<a \<mapsto>\<^sub>a xs * \<up>(l < length xs) * \<up>(r < length xs)>
-   quicksort a l r
-   <\<lambda>rs. \<exists>\<^sub>Axs'. a \<mapsto>\<^sub>a xs' * \<up>(sorted (sublist l (r + 1) xs'))>" by auto2
-
-definition quicksort_all :: "('a::{heap,linorder}) array \<Rightarrow> unit Heap" where
+definition quicksort_all :: "('a::{heap,linorder}) array \<Rightarrow> unit Heap" where [sep_proc_defs]:
   "quicksort_all a = do {
      n \<leftarrow> Array.len a;
      if n = 0 then return ()
      else quicksort a 0 (n - 1) }"
-declare quicksort_all_def [sep_proc_defs]
 
 theorem quicksort_sorts_basic [hoare_triple]:
   "<a \<mapsto>\<^sub>a xs>
    quicksort_all a
-   <\<lambda>_. a \<mapsto>\<^sub>a sort (xs::('a::{heap,linorder}) list)>"
+   <\<lambda>_. a \<mapsto>\<^sub>a sort xs>"
 @proof
-  @case "xs = []" @with
-    @have "sort ([]::'a list) = []" @end
+  @case "xs = []"
   @have "Quicksort.quicksort xs 0 (length xs - 1) = sort xs"
 @qed
 declare quicksort_all_def [sep_proc_defs del]
